Hoare/While/Context.lean
@@ -11,6 +11,7 @@ instance : Coe Nat Val := ⟨Val.num⟩
 instance : Coe Bool Val := ⟨Val.bool⟩
 instance {n : Nat} : CoeDep Val (Val.num n) Nat := ⟨n⟩
 instance {b : Bool} : CoeDep Val (Val.bool b) Bool := ⟨b⟩
+instance : OfNat Val n := ⟨Val.num n⟩
 
 def Val.toExpr : Val → Expr
   | Val.num n => Expr.num n
@@ -37,7 +38,25 @@ def Context.reprPrec : Context → Nat → Std.Format
   | [], _ => Std.Format.nil
   | (x, v) :: ctx, n => x ++ " ↦ " ++ repr v ++ "; " ++ reprPrec ctx n
 
+-- Syntactic sugar
+declare_syntax_cat ctx
+
+syntax  ident " ↦ " term " ;" ctx : ctx
+syntax  ident " ↦ " term : ctx
+syntax "[" ctx "]c" : term
+macro_rules
+  | `([ $x:ident ↦ $v:term ; $c:ctx ]c) =>
+    let xs := Lean.quote x.getId.toString
+    `(List.cons (Prod.mk $xs $v) [$c]c)
+  | `([ $x:ident ↦ $v:term]c) =>
+    let xs := Lean.quote x.getId.toString
+    `(List.cons (Prod.mk $xs $v) List.nil)
+
+
 -- Probably not doing the prec thing right
 instance : Repr Context := ⟨Context.reprPrec⟩
+
+private def testCtxt : Context := [ x ↦ 1]c
+#print testCtxt
 
 end While
